Fix cpc

Cpc/Logos.lean
@@ -6244,7 +6244,7 @@ def __eo_typeof : Term -> Term
   | (Term.Apply (Term.Apply Term.xor __eo_x1) __eo_x2) => (__eo_typeof_or (__eo_typeof __eo_x1) (__eo_typeof __eo_x2))
   | (Term.Apply (Term.Apply Term.eq __eo_x1) __eo_x2) => (__eo_typeof_eq (__eo_typeof __eo_x1) (__eo_typeof __eo_x2))
   | (Term.Apply Term.distinct __eo_x1) => (__eo_typeof_distinct (__eo_typeof __eo_x1))
-  | (Term._at_purify __eo_x1) => (__eo_typeof_Seq (__eo_typeof __eo_x1))
+  | (Term._at_purify __eo_x1) => (__eo_typeof __eo_x1)
   | (Term.Apply (Term.Apply Term.plus __eo_x1) __eo_x2) => (__eo_typeof_plus (__eo_typeof __eo_x1) (__eo_typeof __eo_x2))
   | (Term.Apply (Term.Apply Term.neg __eo_x1) __eo_x2) => (__eo_typeof_plus (__eo_typeof __eo_x1) (__eo_typeof __eo_x2))
   | (Term.Apply (Term.Apply Term.mult __eo_x1) __eo_x2) => (__eo_typeof_plus (__eo_typeof __eo_x1) (__eo_typeof __eo_x2))
